\documentclass[12pt]{ujarticle}
\usepackage{amsmath,amsfonts,amsthm,amssymb,amscd,txfonts}
\usepackage[all]{xy}
\def\objectstyle{\displaystyle}
\begin{document}
\begin{eqnarray}
\Delta f  = \frac{1}{\sqrt{g}}\partial_{\mu}\left(\sqrt{g}g^{\mu\nu}\partial_{\nu}f\right)
\end{eqnarray}
\begin{eqnarray}
ds^2 &=& g_{\mu\nu}dx^{\mu}dx^{\nu} \\
&=& dr^2 + r^2 d\theta^2 + r^2\sin ^2 \theta d\phi^2
\end{eqnarray}
\begin{eqnarray}
g = dr \otimes dr + r^2 d\theta \otimes d\theta + r^2\sin^2\theta d\phi \otimes d\phi
\end{eqnarray}
\begin{eqnarray}
g_{11} = g_{rr} = 1 \\
g_{22} = g_{\theta\theta} = r^2 \\
g_{33} = g_{\phi\phi} = r^2\sin^2\theta
\end{eqnarray}
\begin{eqnarray}
g_{\mu\nu} =
\begin{pmatrix}
1 & 0  & 0\\
0 & r^2 & 0 \\
0 & 0 & r^2\sin^2\theta \\
\end{pmatrix}
\end{eqnarray}
\begin{eqnarray}
\mathrm{det}g_{\mu\nu} = r^4\sin^2\theta
\end{eqnarray}
\begin{eqnarray}
g^{\mu\nu} = \left(g^{-1}\right)_{\mu\nu} =
\begin{pmatrix}
1 & 0 & 0 \\
0 & \frac{1}{r^2} & 0 \\
0 & 0 & \frac{1}{r^2\sin^2\theta} \\
\end{pmatrix}
\end{eqnarray}
\begin{eqnarray}
\sqrt{g} = \sqrt{\left|\mathrm{det}g_{\mu\nu}\right|} = r^2\sin\theta
\end{eqnarray}
\begin{align}
g^{11} = g^{rr} = 1 \\
g^{22} = g^{\theta\theta} = \frac{1}{r^2} \\
g^{33} = g^{\phi\phi} = \frac{1}{r^2\sin^2\theta}
\end{align}
\begin{align}
\Delta f &= \frac{1}{\sqrt{g}}\partial_{\mu}\left(\sqrt{g}g^{\mu\nu}\partial_{\nu}f\right) \\
&= \frac{1}{r^2\sin\theta}\left\{\frac{\partial}{\partial r}\left(r^2\sin\theta g^{rr}\frac{\partial f}{\partial r}\right) + \frac{\partial}{\partial\theta}\left(r^2\sin\theta g^{\theta\theta}\frac{\partial f}{\partial \theta}\right) + \frac{\partial}{\partial \phi}\left(r^2\sin\theta g^{\phi\phi}\frac{\partial f}{\partial \phi}\right)\right\} \\
&= \frac{1}{r^2\sin\theta}\left\{\sin\theta\frac{\partial}{\partial r}\left(r^2\frac{\partial f}{\partial r}\right) + \frac{\partial}{\partial \theta}\left(\sin\theta\frac{\partial f}{\partial \theta}\right) + \frac{1}{\sin\theta}\frac{\partial^2 f}{\partial \phi^2} \right\} \\
&= \frac{1}{r^2}\frac{\partial}{\partial r}\left(r^2\frac{\partial f}{\partial r}\right) + \frac{1}{r^2\sin\theta}\frac{\partial}{\partial \theta}\left(\sin\theta\frac{\partial f}{\partial \theta}\right) + \frac{1}{r^2\sin^2\theta}\frac{\partial^2 f}{\partial \phi^2}
\end{align}




\begin{eqnarray}
\Delta f  = \frac{1}{\sqrt{g}}\partial_{\mu}\left(\sqrt{g}g^{\mu\nu}\partial_{\nu}f\right)
\end{eqnarray}
\begin{eqnarray}
g \coloneqq \left|\mathrm{det}g_{\mu\nu}\right|
\end{eqnarray}
\begin{eqnarray}
\nabla_{\mu}V^{\nu} = \partial_{\mu}V^{\nu} + \Gamma^{\nu}_{\mu\lambda}V^{\lambda}
\end{eqnarray}
\begin{eqnarray}
\Delta f &=& \nabla_{\mu}\left(g^{\mu\nu}\partial_{\nu}f\right) \\
&=& \partial_{\mu}\left(g^{\mu\nu}\partial_{\nu}f\right) + \Gamma^{\mu}_{\mu\lambda}\left(g^{\lambda\nu}\partial_{\nu}f\right) \\
&=& \partial_{\mu}\left(g^{\mu\nu}\partial_{\nu}f\right) + \left(\partial_{\lambda}\log\sqrt{g}\right)\left(g^{\lambda\nu}\partial_{\nu}f\right) \\
&=& \frac{1}{\sqrt{g}}\left\{\sqrt{g}\partial_{\mu}\left(g^{\mu\nu}\partial_{\nu}f\right) + \left(\partial_{\lambda}\sqrt{g}\right)\left(g^{\lambda\nu}\partial_{\nu}f\right)\right\} \\
&=& \frac{1}{\sqrt{g}}\partial_{\mu}\left(\sqrt{g}g^{\mu\nu}\partial_{\nu}f\right)
\end{eqnarray}
\begin{eqnarray}
\Gamma^{\lambda}_{\mu\nu} = \frac{g^{\lambda\rho}}{2}\left(\partial_{\mu}g_{\rho\nu} + \partial_{\nu}g_{\rho\mu} - \partial_{\rho}g_{\mu\nu}\right)
\end{eqnarray}
\begin{eqnarray}
\Gamma^{\mu}_{\mu\lambda} &=& \frac{g^{\mu\rho}}{2}\left(\partial_{\mu}g_{\rho\lambda} + \partial_{\lambda}g_{\rho\mu} - \partial_{\rho}g_{\mu\lambda}\right) \\
&=& \frac{g^{\mu\rho}}{2}\partial_{\lambda}g_{\rho\mu} \\
&=& \frac{\left(g^{-1}\right)_{\mu\rho}}{2}\partial_{\lambda}g_{\rho\mu} \\
&=& \partial_{\lambda}\log\sqrt{g}
\end{eqnarray}





\begin{eqnarray}
A^{-1} = \frac{1}{\mathrm{det}A}\tilde{A}
\end{eqnarray}
\begin{eqnarray}
\left(A^{-1}\right)_{ij} = \frac{1}{\mathrm{det}A}\left(\tilde{A}\right)_{ij}
\end{eqnarray}
\begin{eqnarray}
\mathrm{det}A &=& \sum_{j}A_{ij}\left(\tilde{A}^\top\right)_{ij} \\
&=& \sum_{j}A_{ij}\left(\tilde{A}\right)_{ji}
\end{eqnarray}
\begin{eqnarray}
\frac{\partial \mathrm{det}A}{\partial x^{\mu}} &=& \sum_{i,j}\frac{\partial\mathrm{det}A}{\partial A_{ij}}\frac{\partial A_{ij}}{\partial x^{\mu}} \\
&=& \sum_{i,j}\left(\tilde{A}\right)_{ji}\frac{\partial A_{ij}}{\partial x^{\mu}} \\
&=& \mathrm{det}A\sum_{i,j}\left(A^{-1}\right)_{ji}\frac{\partial A_{ij}}{\partial x^{\mu}}
\end{eqnarray}
\begin{eqnarray}
\sum_{i,j}\left(A^{-1}\right)_{ji}\frac{\partial A_{ij}}{\partial x^{\mu}} &=& \frac{1}{\mathrm{det}A}\frac{\partial\mathrm{det}A}{\partial x^{\mu}} \\
&=& \frac{\partial}{\partial x^{\mu}}\log\left|\mathrm{det}A\right|
\end{eqnarray}
\end{document}
